tests/SignallingCounter/SignallingCounter.v
@@ -109,23 +109,25 @@ Section WithCava.
   Definition counterWithEnable (en : signal Bit) :
                                signal (Vec Bit 8) ->
                                cava (signal (Vec Bit 8)) :=
-    loopDelayEnable en (addN >=> fork2).
+    loopDelaySEnable en addN.
+
+
+  Definition counterWithEnableTop (i_en : signal (Pair (Vec Bit 8) Bit))
+                                  : cava (signal (Vec Bit 8)) :=
+  let '(i, en) := unpair i_en in
+  counterWithEnable en i.
+
 End WithCava.
 
-(* Note that the signalling counter with delay is slightly different than the
-   one above, in that when not enabled it *does* add the input to the current
-   state, and returns this result, but does not save it. The directly defined
-   version of the counter returns the saved (unchanged) state instead of the
-   unsaved addition result. *)
-
 Example counterEnable_ex1:
-  sequential (counterWithEnable
-                (map nat2bool [1;1;1;1;0;0;0;0])
-                (# [1;1;1;1;1;1;1;1])) = # [1;2;3;4;5;5;5;5].
+  sequential (counterWithEnableTop
+                (combine
+                   (# [1;1;1;1;1;1;1;1])
+                   (map nat2bool [1;1;1;1;0;0;0;0]))) = # [1;2;3;4;4;4;4;4].
 Proof. reflexivity. Qed.
 
 Example counterEnable_ex2:
   sequential (counterWithEnable
                 (map nat2bool [0;0;0;1;1;1;0;1])
-                (# [0;1;2;3;4;5;6;7]) ) = # [0;1;2;3;7;12;18;19].
+                (# [0;1;2;3;4;5;6;7]) ) = # [0;0;0;3;7;12;12;19].
 Proof. reflexivity. Qed.
